coq/cclc/clc_context.v
@@ -1,5 +1,5 @@
 From mathcomp Require Import ssreflect ssrbool eqtype ssrnat seq.
-From Coq Require Import ssrfun Program Utf8 Classical.
+From Coq Require Import ssrfun Classical.
 Require Import AutosubstSsr ARS.
 
 Set Implicit Arguments.
